\documentclass[a4paper]{report}

\input{../../../preamble/packages.tex}
\input{../../../preamble/macros.tex}
\input{../../../preamble/environments.tex}

\usepackage{tikz-3dplot}

\title{Intro PDE}
\author{Janik Sperling}

\begin{document}
% \include{lectures/brownian_motion_and_martingale}
% \include{lectures/ito_integration}
% \newpage
% \include{lectures/task4}
% \include{lectures/uebung}
% \include{lectures/appendix}
% \include{lectures/macro}
\begin{align*}
  \abs{Y-Z}_t \le  \abs{Y}_t + \abs{Z}_t
.\end{align*}
Where  for $0 = t_{1}\le \ldots \le t_{n} = t$
\begin{align*}
  \abs{Y}_t = \sum_{i=1}^{n}  \abs{Y_{t_i} - Y_{t_{i-1}}}
.\end{align*}
Lets say we can use the limit structure already
\begin{align*} 
  \abs{Y}_t &= \lim_{n \to \infty}\sum_{i=1}^{n}  \abs{Y_{t_i} - Y_{t_{i-1}}} = \lim_{n \to \infty} \sum_{i=1}^{n} \lim_{m\to \infty} \sum_{J \in  \Pi_m} (\Delta_{J \cap [0,t_i]} X)^2 -  \lim_{m\to \infty} \sum_{J \in  \Pi_m} (\Delta_{J \cap [0,t_{i-1}]} X)^2\\
            &\le  \lim_{n \to \infty} \sum_{i=1}^{n} \lim_{m\to \infty} \sum_{J \in  \Pi_m} (\Delta_{J \cap [0,t_i]} X)^2 \\
            &=  \lim_{n \to \infty} \lim_{m\to \infty}\sum_{i=1}^{n}  \sum_{J \in  \Pi_m} (\Delta_{J \cap [0,t_i]} X)^2 \\
.\end{align*}
bzw. 
\begin{align*}
  \abs{Y}_t  = \lim_{n\to \infty} \sum_{i=1}^{n} \abs{Y_{t_i}-Y_{t_{i-1}}}  &=  \lim_{n\to \infty} \sum_{i=1}^{n} \abs{\braket{X}_{t_i} - \braket{X}_{t_{i-1}}}\\
                                                                            &\myS{(i)}{\le } \lim_{n\to \infty} \sum_{i=1}^{n} \abs{\braket{X}_{t_i}}\\ 
                                                                            &= \sum_{i=1}^{k} \braket{X}_{t_i} + \lim_{n \to \infty}  \sum_{k=1}^{n} \braket{X}_{t_i} \\
                                                                            &= Y_t + 0
.\end{align*}
If we know 
\begin{align*}
  \sum_{i=1}^{\infty} a_i < \infty 
.\end{align*}
Then 
\begin{align*}
  \lim_{k\to \infty} \sum_{i=k}^{\infty} a_i \to 0 
.\end{align*}
\begin{exercise}
 Let $f(t,x) = t*\frac{x^2}{2}$  show 
 \begin{align*}
   f(t,B_t) &= f(0,0) + \int_{\mathbb{R}} \frac{\partial f}{\partial s}(s,B_s) ds + \int_{\Omega } \frac{\partial f}{\partial x} + \frac{1}{2} \int \frac{\partial ^2f}{\partial x^2}   ds
            &= 0 + \int_0^{t} \frac{B_s^2}{2} ds + \int_0^{t} s*B_s dB_s + \frac{1}{2}  \int_0^{t} s ds 
 .\end{align*}
\end{exercise}
\end{document}
