\chapter{Relative Entropy Method}
\section{Problem Definition}
\begin{Definition}
\begin{align*}
  (\text{SDE})\begin{cases}
    &dX_i^n = \frac{1}{N}\sum_{j=1}^{N} \nabla V (X_i^{N}-X_j^{N}  )  dt + \sqrt{2}dW_t^i\\
    &X_i^N(0) = \xi_i \text{ i.i.d } u_{0}(x) \in L^{1} ((1 + \abs{x}^2) dx) 
  \end{cases}
.\end{align*}  
\end{Definition}
\begin{corollary}
Now let $u_N(*,t)$ be the joint law of $(X_1(t)^{N},\ldots ,X_N^{N}(t)   )$, then by It\^o s formula and taking the expectation we know $u_N$ satisfies
\begin{align*}
  \partial_t u_{N} &= \sum_{i=1}^{N} \Delta_{x_i} u_N + \sum_{i=1}^{N} \nabla_{x_i} * (u_N * \frac{1}{N} \sum_{j=1}^{N} \nabla V (X_i^{N}-X_j^{N}  ))\\
  u_{N}\rvert_{t=0} &= u_0^{\otimes N}  = u_{0}(x_{1})u_{0}(x_{2})\ldots u_0(x_N)
.\end{align*}
If $\|\nabla V\|_{\infty} \le C$, then $u_N \in  L^{\infty}([0,T] ; L^{1}(\mathbb{R}^{dN} ) ) $ in addition if $\nabla V$ is "good enough", then $u_N$ is a classical solution
\end{corollary}
\begin{goal}
We want to study what happens as $N\to \infty$, let $u$ be a solution to 
\begin{align*}
  \partial_t u - \Delta u = \nabla * (\nabla V \star  u * u)
.\end{align*}
We expect 
\begin{align*}
  u_N - u^{\otimes N}  \xrightarrow{N\to \infty} 0 
.\end{align*}
where  $u^{\otimes N} $ should satisfy 
\begin{align*}
  \partial_t u^{\otimes N}  = \sum_{i=1}^{N} \Delta _{x_i}  u^{\otimes N}  + \sum_{i=1}^{N} \nabla_{x_i}  * (u^{\otimes N} \nabla V \star u(x_i) )
.\end{align*}
we compare 
\begin{align*}
  \partial_t u_{N} &= \sum_{i=1}^{N} \Delta_{x_i} u_N + \sum_{i=1}^{N} \nabla_{x_i} * (u_N * \frac{1}{N} \sum_{j=1}^{N} \nabla V (X_i^{N}-X_j^{N}  ))\\ 
                   &\hspace{23mm} \text{ and }\\
\partial_t u^{\otimes N}  &= \sum_{i=1}^{N} \Delta _{x_i}  u^{\otimes N}  + \sum_{i=1}^{N} \nabla_{x_i}  * (u^{\otimes N} \nabla V \star u(x_i) )
.\end{align*}
\end{goal}
\section{Entropy}
\begin{definition}[Entropy]
 For the heat equation $\partial_t - \Delta  u = 0$ we have 
 \begin{align*}
   \hspace{-20mm} L^2 :\qquad \frac{d}{dt} \int  u ^2 + \int  \abs{\nabla u}^2  = u
 .\end{align*}
using $\phi  = u \log u$ as a test function then  we get that 
\begin{align*}
  \int_{\mathbb{R}^{d} } \partial_t u \log u - \int_{\mathbb{R}^{d} } \Delta  u \log_u  &= 0\\
  \int_{\mathbb{R}^{d} } \partial_t u \log u + \int  \nabla u \frac{\nabla u}{u} &=0 \\
  \int_{\mathbb{R}^{d} } \partial_t u \log u +   \int (\nabla \sqrt{u} )^2  &=0 \\
  \int_{\mathbb{R}^{d} } \partial_t u \log u +  \int  \abs{\nabla \log u} ^2 u &=0 
.\end{align*}
\textcolor{Red}{Not really sure about the above }
\end{definition}
\begin{definition}[Relative Entropy]
 Relative entropy then means comparing two functions $u_1 \to u_{2}$  
 \begin{align*}
   \partial_t \int_{\mathbb{R}^{d} }\frac{u_{1}}{u_{2}} \log \frac{u_{1}}{u_{2}}*u_{2}(x) dx &= \partial_t \int u_{1} \log \frac{u_{1}}{u_{2}}\\
                                                                                             &= \int_{\mathbb{R}^{d} } \partial_t u_{1} \log \frac{u_{1}}{u_{2}} + \int u_{1} \frac{u_{2}}{u_{1}}(\partial_t \frac{u_{1}}{u_{2}}) 
 .\end{align*}
\end{definition}
\begin{align*}
  \mathcal{H}(u_N | u^{\otimes N}) = \mathcal{H}_N(u_N | u^{\otimes N} ) = \frac{1}{N} \int_{\mathbb{R}^{dN} } \frac{u_N}{u^{\otimes n} } \log \frac{u_N}{u^{\otimes N} } u^{\otimes N}  dx_{1}\ldots dx_N
.\end{align*}
We study
\begin{align*}
  \frac{d}{dt} \mathcal{H}(u_N | u^{\otimes N}) &= \frac{1}{N} \int_{\mathbb{R}^{dN} } \partial_t u_N  \log \frac{u_N}{u^{\otimes N} }d(x_{1},\ldots x_N) + \frac{1}{N} \int u^{\otimes N}  \partial_t (\frac{u_N}{u^{\otimes N} }) d\underbrace{(x_{1},\ldots ,x_N)}_{X_N} \\
                                                &= \frac{1}{N} \int_{\mathbb{R}^{dN} } \partial_t u_N  \log \frac{u_N}{u^{\otimes N} }dX_N + \frac{1}{N} \int \partial_t u_N - u_N \frac{u^{\otimes N}}{(u^{\otimes N} )^2} u^{\otimes N} dX_N\\
                                                &= \frac{1}{N} \int_{\mathbb{R}^{dN} }- \sum_{i=1}^{N}(\nabla_{x_i} u_N + u_N \frac{1}{N} \sum_{j=1}^{N} \nabla V (x_i-x_j) ) \nabla_{x_i} \log \frac{u_N}{u^{\otimes N} } dX_N\\
                                                &\quad - \frac{1}{N} \int_{\mathbb{R}^{dN} }-  \sum_{i=1}^{N}(\nabla_{x_i} u^{\otimes N}  + u^{\otimes N} \nabla V \star u(x_i) ) \underbrace{\nabla_{x_i}(\frac{u_N}{u^{\otimes N} })}_{= \frac{u_N}{u^{\otimes N} }*\nabla_{x_i} \log \frac{u_N}{u^{\otimes N} }}dX_N\\
                                                &= \frac{1}{N} \int_{\mathbb{R}^{dN} } \sum_{i=1}^{N}(-\nabla_{x_i}u_N + \nabla_{x_i} u^{\otimes N}*\frac{u_N}{u^{\otimes N} } ) \nabla_{x_i} \log \frac{u_N}{u^{\otimes N} } dX_N\\
                                                &\quad + \frac{1}{N} \int_{\mathbb{R}^{dN} } \left(\sum_{i=1}^{N} \nabla V \star  u(x_i)  - \frac{1}{N} \sum_{j=1}^{N}  \nabla V(x_i - x_j) \right)u_N \nabla_{x_i} \log \frac{u_N}{u^{\otimes N} } dX_N
.\end{align*}
To summarize 
\begin{align*}
  \frac{d}{dt} \mathcal{H}(u^{N} | u^{\otimes N}  ) &= -   \frac{1}{N} \int_{\mathbb{R}^{dN} } \sum_{i=1}^{N}  \abs*{\nabla_{x_i} \log \frac{u_N}{u^{\otimes N} }}^2 u_N d X_N\\
                                                    &\quad - \frac{1}{N} \sum_{i=1}^{N} \int_{\mathbb{R}^{dN} }  \nabla_{x_i} \log \frac{u_N}{u^{\otimes N} } \left[ u_N \left(\nabla V \star u(x_i) - \frac{1}{N} \sum_{j=1}^{N} \nabla V(x_i-x_j) \right) \right]  dX_N\\
                                                    &\le - \frac{1}{N} \int_{\mathbb{R}^{dN} } \sum_{i=1}^{N} \abs{\nabla_{x_i} \log \frac{u_N}{u^{\otimes N} }}^2 u_N dX_N \\
                                                    &\quad + \frac{1}{2} \int_{\mathbb{R}^{dN} } u_N \frac{1}{N} \sum_{i=1}^{N}  \abs*{\nabla V \star  u (x_i) - \frac{1}{N} \nabla V(x_i-x_j) }^2 dX_N\\
                                                    &= -\frac{1}{2N} \int_{\mathbb{R}^{dN} } \sum_{i=1}^{N} \abs*{\nabla_{x_i} \log  \frac{u_N}{u^{\otimes N} }}^2 u_N dX_N + \frac{1}{2} \E\left[\frac{1}{N} \sum_{i=1}^{N} \abs*{\nabla V \star  u(X_i)-\nabla V \star  \mu_N(X_i)}^2 \right] \marginnote{\footnotesize $X_i$ stochastic}\\
                                                    &= I + II
.\end{align*}
If  for some $\theta  > 0$
\begin{align*}
  II \le   \frac{C}{N^{\theta } }
.\end{align*}
Then  $\mathcal{H}(u_N | u^{\otimes N} ) \le \frac{C}{N^{\theta } } t $. Notice that 
\begin{align*}
  \mathcal{H}(u_N | u^{\otimes N} )\rvert_{t=0}  = 0
.\end{align*}
super-additivity for relative entropy
\begin{align*}
  \mathcal{H}_k (u^{(k)}_N | u^{\otimes k}  ) \le  2k \mathcal{H}(u_N | u^{\otimes N} ) \le \frac{C(k)t}{N^{\theta } }
.\end{align*}
where 
\begin{align*}
  u_N^{(k)}(x_{1},\ldots ,x_k)= \int_{\mathbb{R}^{d(N-k)} }u_N(x_{1},\ldots ,x_N) dx_{k}\ldots dx_N
.\end{align*}
is the $k$-th marginal, now if $k=1$ 
\begin{align*}
  \int_{\mathbb{R}^{d} } u_N^{(1)}  \log \frac{u_N^{(1)} }{u} dx_{1} = \mathcal{H}_1(u_N^{(1)} | u ) \le  \frac{C}{N^{\theta } } \to 0
.\end{align*}
the Csisz\`ar-Kullback-Pinsker inequality says
\begin{align*}
  \|u_N^{(1)}-U \|_{L^2}^{2} \le  2 \mathcal{H}_1(u_{N}^{(1)} | u ) 
.\end{align*}
\begin{lemma}[Csisz\`ar-Kullback-Pinsker]
 For $0\le f,g \in  L^{1}(\mathbb{R}^{d} ) $ the entropy of $f$ and $g$ 
 \begin{align*}
   \mathcal{H}(f | g) = \int_{\mathbb{R}^{d} } f \log \frac{f}{g}
 .\end{align*}
 Where the negative part of $\mathcal{H}(f|g)$
 \begin{align*}
   \int_{f \le g} f * \abs{\log \frac{f}{g}} =  \int_{f \le  g} g \frac{f}{g} \abs{\log  \frac{f}{g}} \le  \frac{1}{e} \|g\|_{L^{1} }
 .\end{align*}
 we used 
 \begin{align*}
  r \log  r \ge  -\frac{1}{e}
 .\end{align*}
 if $\|f\|_{L^{1}} = \|g\|_{L^{1} } $, then
 \begin{align*}
   \int_{\mathbb{R}^{d} } \frac{f}{g} \log  \frac{f}{g} g dx \ge \int  \frac{f}{g} * g dx - \int g dx = 0
 .\end{align*}
 this means for two probability densities ($\|\mu \|_{L^{1} }=\|\nu \|_{L^{1} } = 1$) the entropy is always positive\\[1ex]
 The inequality then states that if $\|f\|_{L^{1} } = \|g\|_{L^{1} }$ it holds 
 \begin{align*}
   \|f-g\|_{L^{1} }^2 \le 2 \mathcal{H}(f | g)
 .\end{align*}
\end{lemma}
\begin{proof}
 We compute 
 \begin{align*}
   \left( \int \abs{f-g} dx \right)^2 &=  \left( \int  \abs{\frac{f}{g} - 1} g  dx\right) ^2\\
                                      &= \left( \int  \frac{\abs{\frac{f}{g} - 1}}{\sqrt{\frac{f}{g} + 2}} g^{\frac{1}{2}}(\sqrt{\frac{f}{g}+2})g^{\frac{1}{2}} dx  \right) ^2\\
                                      &\myS{HÃ¶ld.}{\le } \int \frac{\abs{\frac{f}{g}-1}^2}{(\frac{f}{g}+2)}g dx *\int (\frac{f}{g} + 2)g dx\\
                                      &\le  3 \frac{2}{3} \left( \int \frac{f}{g} \log \frac{f}{g} g dx - \int (\frac{f}{g} - 1) g dx \right) \\
                                      &= 2 \int f \log \frac{f}{g} dx\\
                                      &= 2 \mathcal{H}(f|g)
 .\end{align*}
 since $\|f\|_{L^{1} } = \|g\|_{L^{1} }$ we may assume $\|f\|_{L^1} = 1$ \\
 Where we used 
\begin{align*}
  r \log  r - r + 1 \ge  \frac{3}{2} \frac{(r-1)^2}{r+2} \quad \forall  r \ge 0
.\end{align*}
\end{proof}
\begin{note}
 Two points remain 
 \begin{enumerate}
   \item $\mathcal{H}_k(u_N^{(k)}|u^{\otimes k}  ) \le  C \mathcal{H}_N(u_N | u^{\otimes N} )$
   \item  $\E \left[ \braket{\mu_N,\abs{\nabla V \star (\mu_N - u)}^2} \right] \le  \frac{C}{N^{\theta } } $
 \end{enumerate}
\end{note}
